Start on poly progress, fix WellFormed

proof/Poly/Exp.v
@@ -1,6 +1,6 @@
 
 Require Export Env.
-
+Require Import Base.
 
 (* Kinds ************************************************************)
 Inductive ki : Type :=
@@ -22,6 +22,35 @@ Definition tyenv := env ty.
 Hint Unfold tyenv.
 
 
+(* Lift type indices that are at least a certain depth. *)
+Fixpoint liftTT (d: nat) (tt: ty) : ty :=
+  match tt with
+  | TCon _     => tt
+
+  |  TVar ix
+  => if le_gt_dec d ix
+      then TVar (S ix)
+      else tt
+
+  |  TForall t 
+  => TForall (liftTT (S d) t)
+
+  |  TFun t1 t2
+  => TFun    (liftTT d t1) (liftTT d t2)
+  end.
+Hint Unfold liftTT.
+
+(* Lift type indices in type environments. *)
+Definition liftTE d te    := map (liftTT d) te.
+Hint Unfold liftTE.
+
+Ltac lift_cases 
+ := match goal with 
+     |  [ |- context [le_gt_dec ?n ?n'] ]
+     => case (le_gt_dec n n')
+    end.
+
+
 (** Expressions *****************************************************)
 Inductive exp : Type :=
  | XVar  : nat -> exp
@@ -30,5 +59,28 @@ Inductive exp : Type :=
  | XLam  : ty  -> exp -> exp
  | XApp  : exp -> exp -> exp.
 Hint Constructors exp.
+
+
+(* Lift value indices in expressions.
+   That are greater or equal to a given depth. *)
+Fixpoint liftXX (d: nat) (xx: exp) : exp :=
+  match xx with
+  |  XVar ix    
+  => if le_gt_dec d ix
+      then XVar (S ix)
+      else xx
+
+  |  XLAM x
+  => XLAM (liftXX d x)
+
+  |  XAPP x t
+  => XAPP (liftXX d x) t
+ 
+  |  XLam t x   
+  => XLam t (liftXX (S d) x)
+
+  |  XApp x1 x2
+  => XApp (liftXX d x1) (liftXX d x2)
+ end.
 
 
