proof/Poly/TyJudge.v
@@ -1,6 +1,7 @@
 
 Require Import SubstTypeType.
 Require Import KiJudge.
+Require Import WellFormed.
 Require Import Exp.
 Require Import Env.
 Require Import Base.
@@ -11,11 +12,13 @@ Inductive TYPE : kienv -> tyenv -> exp -> ty -> Prop :=
  | TYVar 
    :  forall i ke te t
    ,  get te i = Some t
+   -> KIND ke t  KStar
    -> TYPE ke te (XVar i) t
 
  | TYLam 
    :  forall ke te x12 t11 t12
-   ,  TYPE ke (te :> t11)  x12            t12
+   ,  KIND ke t11 KStar
+   -> TYPE ke (te :> t11)  x12            t12
    -> TYPE ke  te         (XLam t11 x12) (TFun t11 t12)
 
  | TYApp 
@@ -38,4 +41,55 @@ Inductive TYPE : kienv -> tyenv -> exp -> ty -> Prop :=
 Hint Constructors TYPE.
 
 
+(* Well Formed ******************************************************)
+(* The type produced by a type judgement is well kinded *)
+Theorem type_kind
+ :  forall ke te x t
+ ,  TYPE ke te x t
+ -> KIND ke t KStar.
+Proof.
+ intros. gen ke te t.
+ induction x; intros; inverts H; eauto.
+ 
+ Case "XAPP".
+  apply IHx in H4. inverts H4.
+  eapply subst_type_type; eauto.
+
+ Case "XLam".
+  eapply IHx1 in H4. inverts H4. auto.
+Qed.
+
+
+(* A well typed expression is well formed *)
+Theorem type_wfX
+ :  forall ke te x t
+ ,  TYPE ke te x t
+ -> wfX  ke te x.
+Proof.
+ intros. gen ke te t.
+ induction x; intros; simpl.
+
+ Case "XVar".
+  inverts H. eauto.
+
+ Case "XLAM".
+  inverts H.
+  apply IHx in H3. eauto.
+
+ Case "XAPP".
+  inverts H. 
+  lets D: IHx H4. split. 
+   auto. eapply kind_wfT. eauto.
+
+ Case "XLam".
+  inverts H.
+  apply IHx in H6.
+  apply kind_wfT in H4. auto.
+
+ Case "XApp".
+  inverts H.
+  apply IHx1 in H4. 
+  apply IHx2 in H6.
+   auto.
+Qed.
 
