proof/Poly/EsJudge.v
@@ -1,0 +1,37 @@
+
+Require Import SubstTypeValue.
+Require Import SubstValueValue.
+Require Import WellFormed.
+Require Import Exp.
+
+
+(* Single Step Evaluation *******************************************)
+Inductive STEP : exp -> exp -> Prop := 
+  (* value applications *)
+  | ESLamApp
+    :  forall t11 x12 v2
+    ,  value v2
+    -> STEP (XApp (XLam t11 x12) v2) (substXX 0 v2 x12)
+
+  | ESApp1
+    :  forall x1 x1' x2
+    ,  STEP x1 x1'
+    -> STEP (XApp x1 x2) (XApp x1' x2)
+ 
+  | ESApp2
+    :  forall v1 x2 x2'
+    ,  value v1
+    -> STEP x2 x2'
+    -> STEP (XApp v1 x2) (XApp v1 x2')
+
+  (* type applications *)
+  | ESLAMAPP
+    :  forall x12 t2      
+    ,  STEP (XAPP (XLAM x12) t2) (substTX 0 t2 x12)
+
+  | ESAPP1
+    :  forall x1 x1' t2
+    ,  STEP (XAPP x1 t2) (XAPP x1' t2).
+
+
+        
