proof/Poly/Progress.v
@@ -1,0 +1,23 @@
+
+
+Require Import WellFormed.
+Require Import EsJudge.
+Require Import TyJudge.
+Require Import Exp.
+Require Import Base.
+
+
+Theorem Progress
+ :  forall x t
+ ,  TYPE Empty Empty x t
+ -> value x \/ (exists x', STEP x x').
+Proof.
+ intros.
+ induction x.
+
+ Case "XVar".
+  inverts H. false.
+
+ Case "XLAM".
+  left. apply Value_LAM.
+  inverts H.
